theories/ZX/VyZXHyperGraph.v
@@ -1,0 +1,46 @@
+Require Export VyZXTensor.
+From stdpp Require Import vector. 
+Require Import TensorGraph TensorGraphSemantics 
+  TensorGraphFacts GraphRewriting ZXGraph.
+
+
+Fixpoint ZX_graph_semantics {n m} (zx : ZX n m) : 
+  @CospanHyperGraph (option (bool * R)) n m :=
+  match zx with 
+  | ⦰ => id_graph 0
+  | ⊂ => cup_graph 1
+  | ⊃ => cap_graph 1
+  | ⨉ => swap_graph 1 1
+  | — => id_graph 1
+  | □ => graph_of_tensor None 1 1
+  | X n m α => graph_of_tensor (Some (true, α)) n m
+  | Z n m α => graph_of_tensor (Some (false, α)) n m
+  | zx0 ↕ zx1 => stack_graphs (ZX_graph_semantics zx0) (ZX_graph_semantics zx1)
+  | zx0 ⟷ zx1 => compose_safe (ZX_graph_semantics zx0) (ZX_graph_semantics zx1)
+  end.
+
+
+
+
+Lemma ZX_graph_semantics_correct {n m} (zx : ZX n m) :
+  graph_semantics (ZX_graph_semantics zx) ≡ ZX_tensor_semantics zx.
+Proof.
+  induction zx.
+  - cbn.
+    apply graph_semantics_id.
+  - apply graph_semantics_cup_1_1.
+  - apply graph_semantics_cap_1_1.
+  - apply graph_semantics_swap_1_1.
+  - apply graph_semantics_id.
+  - cbn.
+    rewrite graph_semantics_graph_of_tensor.
+    apply h_stack1'_11.
+  - refine (graph_semantics_graph_of_tensor _ _ _).
+  - refine (graph_semantics_graph_of_tensor _ _ _).
+  - cbn.
+    rewrite graph_semantics_stack_graphs.
+    now apply stack_tensor_mor.
+  - cbn.
+    rewrite graph_semantics_compose_safe.
+    now apply compose_tensor_mor.
+Qed.
